git-svn-id: https://projects.brucker.ch/hol-testgen/svn/HOL-TestGen/trunk/hol-testgen@9407 3260e6d1-4efc-4170-b0a7-36055960796d

examples/OCL_linked_list.thy
@@ -18,7 +18,7 @@ of the compilation informally, an present a concrete example which is verified i
 
 section{* Outlining the Example *}
 
-section{* Example Data-Universe *}
+section{* Example Data-Universe and its Infrastructure *}
 text{* Should be generated entirely from a class-diagram. *}
 
 (* @{text "'\<AA>"} -- \mathfrak{A} *)
@@ -26,12 +26,12 @@ text{* Our data universe  consists in the concrete class diagram just of node's,
 and implicitly of the class object. Each class implies the existence of a class 
 type defined for the corresponding object representations as follows: *}
 
-datatype node =  mk_Node   oid (* the oid to the node itself *)
-                           "int option" (* the attribute "i" or null *) 
-                           "oid option" (* the attribute "next" or null *)
+datatype node =  mk\<^isub>n\<^isub>o\<^isub>d\<^isub>e   oid          (* the oid to the node itself *)
+                         "int option" (* the attribute "i" or null *) 
+                         "oid option" (* the attribute "next" or null *)
 
 
-datatype object= mk_Object oid (* the oid to the object itself *)
+datatype object= mk\<^isub>o\<^isub>b\<^isub>j\<^isub>e\<^isub>c\<^isub>t oid (* the oid to the object itself *)
                            "(int option \<times> oid option) option" 
                            (* the extensions to "node"; used to denote objects of actual type
                              "node" casted to "object"; in case of existence of several subclasses 
@@ -40,16 +40,16 @@ datatype object= mk_Object oid (* the oid to the object itself *)
 text{* Now, we construct a concrete "universe of object types" by injection into a 
 sum type containing the class types. This type of objects will be used as instance
 for all resp. type-variables ...*}
-datatype \<AA> = mk\<^isub>n\<^isub>o\<^isub>d\<^isub>e node | mk\<^isub>o\<^isub>b\<^isub>j\<^isub>e\<^isub>c\<^isub>t object
+datatype \<AA> = in\<^isub>n\<^isub>o\<^isub>d\<^isub>e node | in\<^isub>o\<^isub>b\<^isub>j\<^isub>e\<^isub>c\<^isub>t object
 
 text{* Recall that in order to denote OCL-types occuring in OCL expressions syntactically 
 --- as, for example,  as "argument" of allInstances --- we use the inverses of the injection 
 functions into the object universes; we show that this is sufficient "characterization". *}
 definition Node :: "\<AA> \<Rightarrow> node"
-where     "Node \<equiv> (the_inv mk\<^isub>n\<^isub>o\<^isub>d\<^isub>e)"
+where     "Node \<equiv> (the_inv in\<^isub>n\<^isub>o\<^isub>d\<^isub>e)"
 
 definition Object :: "\<AA> \<Rightarrow> object"
-where     "Object \<equiv> (the_inv mk\<^isub>o\<^isub>b\<^isub>j\<^isub>e\<^isub>c\<^isub>t)"
+where     "Object \<equiv> (the_inv in\<^isub>o\<^isub>b\<^isub>j\<^isub>e\<^isub>c\<^isub>t)"
 
 
 text{* Having fixed the object universe, we can introduce type synonyms that exactly correspond
@@ -71,21 +71,21 @@ to show that the object universe belongs to the type class "object", i.e. each c
 has to provide a function @{term oid_of} yielding the object id (oid) of the object. *}
 instantiation node :: object
 begin
-   definition oid_of_node_def: "oid_of x = (case x of mk_Node oid _ _ \<Rightarrow> oid)"
+   definition oid_of_node_def: "oid_of x = (case x of mk\<^isub>n\<^isub>o\<^isub>d\<^isub>e oid _ _ \<Rightarrow> oid)"
    instance ..
 end
 
 instantiation object :: object
 begin
-   definition oid_of_object_def: "oid_of x = (case x of mk_Object oid _ \<Rightarrow> oid)"
+   definition oid_of_object_def: "oid_of x = (case x of mk\<^isub>o\<^isub>b\<^isub>j\<^isub>e\<^isub>c\<^isub>t oid _ \<Rightarrow> oid)"
    instance ..
 end
 
 instantiation \<AA> :: object
 begin
    definition oid_of_\<AA>_def: "oid_of x = (case x of 
-                                             mk\<^isub>n\<^isub>o\<^isub>d\<^isub>e node \<Rightarrow> oid_of node
-                                           | mk\<^isub>o\<^isub>b\<^isub>j\<^isub>e\<^isub>c\<^isub>t obj \<Rightarrow> oid_of obj)"
+                                             in\<^isub>n\<^isub>o\<^isub>d\<^isub>e node \<Rightarrow> oid_of node
+                                           | in\<^isub>o\<^isub>b\<^isub>j\<^isub>e\<^isub>c\<^isub>t obj \<Rightarrow> oid_of obj)"
    instance ..
 end
 
@@ -96,35 +96,60 @@ begin
 end
 
 
-section{* Instantiation of the generic strict equality *}
-text{* Should be generated entirely from a class-diagram. *}
 
-defs   StrictRefEq_node : "(x::Node) \<doteq> y \<equiv> gen_ref_eq x y"
+section{* Instantiation of the generic strict equality. We instantiate the referential equality
+on @{text "Node"} and @{text "Object"} *}
+
+defs(overloaded)   StrictRefEq\<^isub>n\<^isub>o\<^isub>d\<^isub>e   :  "(x::Node) \<doteq> y    \<equiv> gen_ref_eq x y"
+defs(overloaded)   StrictRefEq\<^isub>o\<^isub>b\<^isub>j\<^isub>e\<^isub>c\<^isub>t  : "(x::Object) \<doteq> y  \<equiv> gen_ref_eq x y"
 
 lemmas strict_eq_node =
     cp_gen_ref_eq_object[of "x::Node" "y::Node" "\<tau>", 
-                         simplified StrictRefEq_node[symmetric]]
+                         simplified StrictRefEq\<^isub>n\<^isub>o\<^isub>d\<^isub>e[symmetric]]
     cp_intro(9)         [of "P::Node \<Rightarrow>Node""Q::Node \<Rightarrow>Node",
-                         simplified StrictRefEq_node[symmetric] ]
+                         simplified StrictRefEq\<^isub>n\<^isub>o\<^isub>d\<^isub>e[symmetric] ]
     gen_ref_eq_def      [of "x::Node" "y::Node", 
-                         simplified StrictRefEq_node[symmetric]]
+                         simplified StrictRefEq\<^isub>n\<^isub>o\<^isub>d\<^isub>e[symmetric]]
     gen_ref_eq_defargs  [of _ "x::Node" "y::Node", 
-                         simplified StrictRefEq_node[symmetric]]
+                         simplified StrictRefEq\<^isub>n\<^isub>o\<^isub>d\<^isub>e[symmetric]]
     gen_ref_eq_object_strict1 
                         [of "x::Node",
-                         simplified StrictRefEq_node[symmetric]]
+                         simplified StrictRefEq\<^isub>n\<^isub>o\<^isub>d\<^isub>e[symmetric]]
     gen_ref_eq_object_strict2 
                         [of "x::Node",
-                         simplified StrictRefEq_node[symmetric]]
+                         simplified StrictRefEq\<^isub>n\<^isub>o\<^isub>d\<^isub>e[symmetric]]
     gen_ref_eq_object_strict3 
                         [of "x::Node",
-                         simplified StrictRefEq_node[symmetric]]
+                         simplified StrictRefEq\<^isub>n\<^isub>o\<^isub>d\<^isub>e[symmetric]]
     gen_ref_eq_object_strict3 
                         [of "x::Node",
-                         simplified StrictRefEq_node[symmetric]]
+                         simplified StrictRefEq\<^isub>n\<^isub>o\<^isub>d\<^isub>e[symmetric]]
     gen_ref_eq_object_strict4 
                         [of "x::Node",
-                         simplified StrictRefEq_node[symmetric]]
+                         simplified StrictRefEq\<^isub>n\<^isub>o\<^isub>d\<^isub>e[symmetric]]
+
+(* TODO: Analogue for object. *)
+
+section{* AllInstances *}
+
+(* IS THIS WHAT WE WANT ? THIS DEFINITION FILTERS OBJECTS THAT ARE BOOKED UNDER
+THEIR APPARENT (STATIC) TYPE INTO THE CONTEXT, NOT BY THEIR ACTUAL (DYNAMIC) TYPE. *)
+lemma "(Node .oclAllInstances()) = 
+             (\<lambda>\<tau>.  Abs_Set_0 \<lfloor>\<lfloor>(Some \<circ> Some \<circ> (the_inv in\<^isub>n\<^isub>o\<^isub>d\<^isub>e))`(ran(snd \<tau>)) \<rfloor>\<rfloor>) "
+by(rule ext, simp add:allinstances_def Node_def)
+
+lemma "(Object .oclAllInstances@pre()) = 
+             (\<lambda>\<tau>.  Abs_Set_0 \<lfloor>\<lfloor>(Some \<circ> Some \<circ> (the_inv in\<^isub>o\<^isub>b\<^isub>j\<^isub>e\<^isub>c\<^isub>t))`(ran(fst \<tau>)) \<rfloor>\<rfloor>) "
+by(rule ext, simp add:allinstancesATpre_def Object_def)
+
+
+text{* For each Class \emph{C}, we will have an casting operation \verb+.oclAsType(+\emph{C}\verb+)+,
+   a test on the actual type \verb+.oclIsTypeOf(+\emph{C}\verb+)+ as well as its relaxed form
+   \verb+.oclIsKindOf(+\emph{C}\verb+)+ (corresponding exactly to Java's \verb+instanceof+-operator. 
+*}
+text{* Thus, since we have two class-types in our concrete class hierarchy, we have
+two operations to declare and and to provide two overloading definitions for the two static types.
+*}
 
 
 section{* Selector Definition *}
@@ -135,12 +160,12 @@ fun dot_next:: "Node \<Rightarrow> Node"  ("(1(_).next)" 50)
   where "(X).next = (\<lambda> \<tau>. case X \<tau> of
                \<bottom> \<Rightarrow> invalid \<tau>           (* undefined pointer *)
           | \<lfloor>  \<bottom> \<rfloor> \<Rightarrow> invalid \<tau>         (* dereferencing null pointer *)
-          | \<lfloor>\<lfloor> mk_Node oid i \<bottom> \<rfloor>\<rfloor> \<Rightarrow> null \<tau>(* object contains null pointer *)
-          | \<lfloor>\<lfloor> mk_Node oid i \<lfloor>next\<rfloor> \<rfloor>\<rfloor> \<Rightarrow>   (* We assume here that oid is indeed 'the' oid of the Node,
+          | \<lfloor>\<lfloor> mk\<^isub>n\<^isub>o\<^isub>d\<^isub>e oid i \<bottom> \<rfloor>\<rfloor> \<Rightarrow> null \<tau>(* object contains null pointer *)
+          | \<lfloor>\<lfloor> mk\<^isub>n\<^isub>o\<^isub>d\<^isub>e oid i \<lfloor>next\<rfloor> \<rfloor>\<rfloor> \<Rightarrow>   (* We assume here that oid is indeed 'the' oid of the Node,
                                            ie. we assume that  \<tau> is well-formed. *)
                     case (snd \<tau>) next of
                        \<bottom> \<Rightarrow> invalid \<tau> 
-                    |  \<lfloor>mk\<^isub>n\<^isub>o\<^isub>d\<^isub>e (mk_Node a b c)\<rfloor> \<Rightarrow> \<lfloor>\<lfloor>mk_Node a b c \<rfloor>\<rfloor>
+                    | \<lfloor>in\<^isub>n\<^isub>o\<^isub>d\<^isub>e (mk\<^isub>n\<^isub>o\<^isub>d\<^isub>e a b c)\<rfloor> \<Rightarrow> \<lfloor>\<lfloor>mk\<^isub>n\<^isub>o\<^isub>d\<^isub>e a b c \<rfloor>\<rfloor>
                     | \<lfloor> _ \<rfloor>\<Rightarrow> invalid \<tau>)" (* illtyped state, not occuring in 
                                              well-formed, typed states *)
 
@@ -148,34 +173,34 @@ fun dot_i:: "Node \<Rightarrow> Integer"  ("(1(_).i)" 50)
   where "(X).i = (\<lambda> \<tau>. case X \<tau> of
                \<bottom> \<Rightarrow> invalid \<tau> 
           | \<lfloor>  \<bottom> \<rfloor> \<Rightarrow> invalid \<tau> 
-          | \<lfloor>\<lfloor> mk_Node oid \<bottom> _ \<rfloor>\<rfloor> \<Rightarrow>  null \<tau>
-          | \<lfloor>\<lfloor> mk_Node oid \<lfloor>i\<rfloor> _ \<rfloor>\<rfloor> \<Rightarrow>  \<lfloor>\<lfloor> i \<rfloor>\<rfloor>)"
+          | \<lfloor>\<lfloor> mk\<^isub>n\<^isub>o\<^isub>d\<^isub>e oid \<bottom> _ \<rfloor>\<rfloor> \<Rightarrow>  null \<tau>
+          | \<lfloor>\<lfloor> mk\<^isub>n\<^isub>o\<^isub>d\<^isub>e oid \<lfloor>i\<rfloor> _ \<rfloor>\<rfloor> \<Rightarrow>  \<lfloor>\<lfloor> i \<rfloor>\<rfloor>)"
 
 fun dot_next_at_pre:: "Node \<Rightarrow> Node"  ("(1(_).next@pre)" 50)
   where "(X).next@pre = (\<lambda> \<tau>. case X \<tau> of
                \<bottom> \<Rightarrow> invalid \<tau>  
           | \<lfloor>  \<bottom> \<rfloor> \<Rightarrow> invalid \<tau> 
-          | \<lfloor>\<lfloor> mk_Node oid i \<bottom> \<rfloor>\<rfloor> \<Rightarrow> null \<tau>(* object contains null pointer. REALLY ? 
+          | \<lfloor>\<lfloor> mk\<^isub>n\<^isub>o\<^isub>d\<^isub>e oid i \<bottom> \<rfloor>\<rfloor> \<Rightarrow> null \<tau>(* object contains null pointer. REALLY ? 
                                           And if this pointer was defined in the pre-state ?*)
-          | \<lfloor>\<lfloor> mk_Node oid i \<lfloor>next\<rfloor> \<rfloor>\<rfloor> \<Rightarrow> (* We assume here that oid is indeed 'the' oid of the Node,
+          | \<lfloor>\<lfloor> mk\<^isub>n\<^isub>o\<^isub>d\<^isub>e oid i \<lfloor>next\<rfloor> \<rfloor>\<rfloor> \<Rightarrow> (* We assume here that oid is indeed 'the' oid of the Node,
                                         ie. we assume that  \<tau> is well-formed. *)
                  (case (fst \<tau>) next of
                         \<bottom> \<Rightarrow> invalid \<tau> 
-                     | \<lfloor>mk\<^isub>n\<^isub>o\<^isub>d\<^isub>e (mk_Node a b c)\<rfloor> \<Rightarrow> \<lfloor>\<lfloor>mk_Node a b c \<rfloor>\<rfloor>
+                     | \<lfloor>in\<^isub>n\<^isub>o\<^isub>d\<^isub>e (mk\<^isub>n\<^isub>o\<^isub>d\<^isub>e a b c)\<rfloor> \<Rightarrow> \<lfloor>\<lfloor>mk\<^isub>n\<^isub>o\<^isub>d\<^isub>e a b c \<rfloor>\<rfloor>
                      | \<lfloor> _ \<rfloor>\<Rightarrow> invalid \<tau>))"
 
 fun dot_i_at_pre:: "Node \<Rightarrow> Integer"  ("(1(_).i@pre)" 50)
 where "(X).i@pre = (\<lambda> \<tau>. case X \<tau> of
               \<bottom> \<Rightarrow> invalid \<tau>
           | \<lfloor>  \<bottom> \<rfloor> \<Rightarrow> invalid \<tau>
-          | \<lfloor>\<lfloor> mk_Node oid _ _ \<rfloor>\<rfloor> \<Rightarrow> 
+          | \<lfloor>\<lfloor> mk\<^isub>n\<^isub>o\<^isub>d\<^isub>e oid _ _ \<rfloor>\<rfloor> \<Rightarrow> 
                       if oid \<in> dom (fst \<tau>)
                       then (case (fst \<tau>) oid of
                                 \<bottom> \<Rightarrow> invalid \<tau>
-                            | \<lfloor>mk\<^isub>n\<^isub>o\<^isub>d\<^isub>e (mk_Node oid \<bottom> next) \<rfloor> \<Rightarrow> null \<tau>
-                            | \<lfloor>mk\<^isub>n\<^isub>o\<^isub>d\<^isub>e (mk_Node oid \<lfloor>i\<rfloor>next) \<rfloor> \<Rightarrow> \<lfloor>\<lfloor> i \<rfloor>\<rfloor>
+                            | \<lfloor>in\<^isub>n\<^isub>o\<^isub>d\<^isub>e (mk\<^isub>n\<^isub>o\<^isub>d\<^isub>e oid \<bottom> next) \<rfloor> \<Rightarrow> null \<tau>
+                            | \<lfloor>in\<^isub>n\<^isub>o\<^isub>d\<^isub>e (mk\<^isub>n\<^isub>o\<^isub>d\<^isub>e oid \<lfloor>i\<rfloor>next) \<rfloor> \<Rightarrow> \<lfloor>\<lfloor> i \<rfloor>\<rfloor>
                             | \<lfloor> _ \<rfloor>\<Rightarrow> invalid \<tau>)
-                      else None)"
+                      else invalid \<tau>)"
 
 lemma cp_dot_next: "((X).next) \<tau> = ((\<lambda>_. X \<tau>).next) \<tau>" by(simp)
 
@@ -198,51 +223,106 @@ by(rule ext, simp add: null_fun_def null_option_def bot_option_def null_def inva
 lemma dot_next_at_pre_nullstrict [simp] : "(null).next@pre = invalid"
 by(rule ext, simp add: null_fun_def null_option_def bot_option_def null_def invalid_def)
 
-lemma dot_next_strict[simp] : "(invalid).next = invalid"
+lemma dot_next_strict[simp] : "(invalid).next = invalid" 
 by(rule ext, simp add: null_fun_def null_option_def bot_option_def null_def invalid_def)
+
+lemma dot_next_strict'[simp] : "(null).next = invalid"
+by(rule ext, simp add: null_fun_def null_option_def bot_option_def null_def invalid_def)
+
 
 lemma dot_nextATpre_strict[simp] : "(invalid).next@pre = invalid"
 by(rule ext, simp add: null_fun_def null_option_def bot_option_def null_def invalid_def)
 
-
-(* IS THIS WHAT WE WANT ? THIS DEFINITION FILTERS OBJECTS THAT ARE BOOKED UNDER
-THEIR APPARENT (STATIC) TYPE INTO THE CONTEXT, NOT BY THEIR ACTUAL (DYNAMIC) TYPE. *)
-lemma "(Node ::oclAllInstances()) = 
-             (\<lambda>\<tau>.  Abs_Set_0 \<lfloor>\<lfloor>(Some \<circ> Some \<circ> (the_inv mk\<^isub>n\<^isub>o\<^isub>d\<^isub>e))`(ran(snd \<tau>)) \<rfloor>\<rfloor>) "
-by(rule ext, simp add:allinstances_def Node_def)
-
-lemma "(Object ::oclAllInstances@pre()) = 
-             (\<lambda>\<tau>.  Abs_Set_0 \<lfloor>\<lfloor>(Some \<circ> Some \<circ> (the_inv mk\<^isub>o\<^isub>b\<^isub>j\<^isub>e\<^isub>c\<^isub>t))`(ran(fst \<tau>)) \<rfloor>\<rfloor>) "
-by(rule ext, simp add:allinstancesATpre_def Object_def)
+lemma dot_nextATpre_strict'[simp] : "(null).next@pre = invalid"
+by(rule ext, simp add: null_fun_def null_option_def bot_option_def null_def invalid_def)
 
 
-text{* For each Class \emph{C}, we will have an casting operation \verb+.oclAsType(+\emph{C}\verb+)+,
-   a test on the actual type \verb+.oclIsTypeOf(+\emph{C}\verb+)+ as well as its relaxed form
-   \verb+.oclIsKindOf(+\emph{C}\verb+)+ (corresponding exactly to Java's \verb+instanceof+-operator. 
-*}
-text{* Thus, since we have two class-types in our concrete class hierarchy, we have
-two operations to declare and and to provide two overloading definitions for the two static types.
-*}
+section{* Casts *}
 
-consts oclastype\<^isub>o\<^isub>b\<^isub>j\<^isub>e\<^isub>c\<^isub>t :: "'\<alpha> \<Rightarrow> Boolean" ("(_).oclAsType'(Object')")
-consts oclastype\<^isub>n\<^isub>o\<^isub>d\<^isub>e   :: "'\<alpha> \<Rightarrow> Boolean" ("(_).oclAsType'(Node')")
+consts oclastype\<^isub>o\<^isub>b\<^isub>j\<^isub>e\<^isub>c\<^isub>t :: "'\<alpha> \<Rightarrow> Object" ("(_).oclAsType'(Object')")
+consts oclastype\<^isub>n\<^isub>o\<^isub>d\<^isub>e   :: "'\<alpha> \<Rightarrow> Node" ("(_).oclAsType'(Node')")
 
-definition oclastype\<^isub>o\<^isub>b\<^isub>j\<^isub>e\<^isub>c\<^isub>t :: "Object \<Rightarrow> Boolean"
-where "X .oclAsType(Object) \<equiv> true"
+defs (overloaded) oclastype\<^isub>o\<^isub>b\<^isub>j\<^isub>e\<^isub>c\<^isub>t_Object: 
+        "(X::Object) .oclAsType(Object) \<equiv> 
+                   (\<lambda>\<tau>. case X \<tau> of 
+                              \<bottom>   \<Rightarrow> invalid \<tau>
+                            | \<lfloor>\<bottom>\<rfloor> \<Rightarrow> invalid \<tau>   (* to avoid: null .oclAsType(Object) = null ? *)
+                            | \<lfloor>\<lfloor>mk\<^isub>o\<^isub>b\<^isub>j\<^isub>e\<^isub>c\<^isub>t oid a \<rfloor>\<rfloor> \<Rightarrow>  \<lfloor>\<lfloor>mk\<^isub>o\<^isub>b\<^isub>j\<^isub>e\<^isub>c\<^isub>t oid a \<rfloor>\<rfloor>)"  (* identity *)
 
-(* MISSING: 
-The instances for 
-consts oclastype 
-consts oclistype
-consts ocliskind
+defs (overloaded) oclastype\<^isub>o\<^isub>b\<^isub>j\<^isub>e\<^isub>c\<^isub>t_Node:  
+        "(X::Node) .oclAsType(Object) \<equiv> 
+                   (\<lambda>\<tau>. case X \<tau> of 
+                              \<bottom>   \<Rightarrow> invalid \<tau>
+                            | \<lfloor>\<bottom>\<rfloor> \<Rightarrow> invalid \<tau>    (* OTHER POSSIBILITY : null ??? Really excluded 
+                                                     by standard *)
+                            | \<lfloor>\<lfloor>mk\<^isub>n\<^isub>o\<^isub>d\<^isub>e oid a b \<rfloor>\<rfloor> \<Rightarrow>  \<lfloor>\<lfloor>  (mk\<^isub>o\<^isub>b\<^isub>j\<^isub>e\<^isub>c\<^isub>t oid \<lfloor>(a,b)\<rfloor>) \<rfloor>\<rfloor>)"
 
+defs (overloaded) oclastype\<^isub>n\<^isub>o\<^isub>d\<^isub>e_Object: 
+        "(X::Object) .oclAsType(Node) \<equiv> 
+                   (\<lambda>\<tau>. case X \<tau> of 
+                              \<bottom>   \<Rightarrow> invalid \<tau>
+                            | \<lfloor>\<bottom>\<rfloor> \<Rightarrow> invalid \<tau>   
+                            | \<lfloor>\<lfloor>mk\<^isub>o\<^isub>b\<^isub>j\<^isub>e\<^isub>c\<^isub>t oid \<bottom> \<rfloor>\<rfloor> \<Rightarrow>  invalid \<tau>   (* down-cast exception *)
+                            | \<lfloor>\<lfloor>mk\<^isub>o\<^isub>b\<^isub>j\<^isub>e\<^isub>c\<^isub>t oid \<lfloor>(a,b)\<rfloor> \<rfloor>\<rfloor> \<Rightarrow>  \<lfloor>\<lfloor>mk\<^isub>n\<^isub>o\<^isub>d\<^isub>e oid a b \<rfloor>\<rfloor>)" 
 
+defs (overloaded) oclastype\<^isub>n\<^isub>o\<^isub>d\<^isub>e_Node: 
+        "(X::Node) .oclAsType(Node) \<equiv> 
+                   (\<lambda>\<tau>. case X \<tau> of 
+                              \<bottom>   \<Rightarrow> invalid \<tau>
+                            | \<lfloor>\<bottom>\<rfloor> \<Rightarrow> invalid \<tau>   (* to avoid: null .oclAsType(Object) = null ? *)
+                            | \<lfloor>\<lfloor>mk\<^isub>n\<^isub>o\<^isub>d\<^isub>e oid a b \<rfloor>\<rfloor> \<Rightarrow>  \<lfloor>\<lfloor>mk\<^isub>n\<^isub>o\<^isub>d\<^isub>e oid a b\<rfloor>\<rfloor>)"  (* identity *)
+
+lemma oclastype\<^isub>o\<^isub>b\<^isub>j\<^isub>e\<^isub>c\<^isub>t_Object_strict[simp] : "(invalid::Object) .oclAsType(Object) = invalid" 
+by(rule ext, simp add: null_fun_def null_option_def bot_option_def null_def invalid_def
+                       oclastype\<^isub>o\<^isub>b\<^isub>j\<^isub>e\<^isub>c\<^isub>t_Object)
+
+lemma oclastype\<^isub>o\<^isub>b\<^isub>j\<^isub>e\<^isub>c\<^isub>t_Object_nullstrict[simp] : "(null::Object) .oclAsType(Object) = invalid" 
+by(rule ext, simp add: null_fun_def null_option_def bot_option_def null_def invalid_def
+                       oclastype\<^isub>o\<^isub>b\<^isub>j\<^isub>e\<^isub>c\<^isub>t_Object)
+
+(* TODO: Missing strictness for other defs, + cp's.*)
+section{* Tests for Actual Types *}
+
+consts oclistypeof\<^isub>o\<^isub>b\<^isub>j\<^isub>e\<^isub>c\<^isub>t :: "'\<alpha> \<Rightarrow> Boolean" ("(_).oclIsTypeOf'(Object')")
+consts oclistypeof\<^isub>n\<^isub>o\<^isub>d\<^isub>e   :: "'\<alpha> \<Rightarrow> Boolean" ("(_).oclIsTypeOf'(Node')")
+
+defs (overloaded) oclistypeof\<^isub>o\<^isub>b\<^isub>j\<^isub>e\<^isub>c\<^isub>t_Object: 
+        "(X::Object) .oclIsTypeOf(Object) \<equiv> 
+                   (\<lambda>\<tau>. case X \<tau> of 
+                              \<bottom>   \<Rightarrow> invalid \<tau>
+                            | \<lfloor>\<bottom>\<rfloor> \<Rightarrow> invalid \<tau>  
+                            | \<lfloor>\<lfloor>mk\<^isub>o\<^isub>b\<^isub>j\<^isub>e\<^isub>c\<^isub>t oid \<bottom> \<rfloor>\<rfloor> \<Rightarrow> true \<tau>
+                            | \<lfloor>\<lfloor>mk\<^isub>o\<^isub>b\<^isub>j\<^isub>e\<^isub>c\<^isub>t oid \<lfloor>_\<rfloor> \<rfloor>\<rfloor> \<Rightarrow> false \<tau>)" 
+
+defs (overloaded) oclistypeof\<^isub>o\<^isub>b\<^isub>j\<^isub>e\<^isub>c\<^isub>t_Node: 
+        "(X::Node) .oclIsTypeOf(Object) \<equiv> 
+                   (\<lambda>\<tau>. case X \<tau> of 
+                              \<bottom>   \<Rightarrow> invalid \<tau>
+                            | \<lfloor>\<bottom>\<rfloor> \<Rightarrow> invalid \<tau>  
+                            | \<lfloor>\<lfloor> _ \<rfloor>\<rfloor> \<Rightarrow> false \<tau>)"  (* must have actual type Node otherwise  *)
+
+defs (overloaded) oclistypeof\<^isub>n\<^isub>o\<^isub>d\<^isub>e_Object: 
+        "(X::Object) .oclIsTypeOf(Node) \<equiv> 
+                   (\<lambda>\<tau>. case X \<tau> of 
+                              \<bottom>   \<Rightarrow> invalid \<tau>
+                            | \<lfloor>\<bottom>\<rfloor> \<Rightarrow> invalid \<tau>  
+                            | \<lfloor>\<lfloor>mk\<^isub>o\<^isub>b\<^isub>j\<^isub>e\<^isub>c\<^isub>t oid \<bottom> \<rfloor>\<rfloor> \<Rightarrow> false \<tau>
+                            | \<lfloor>\<lfloor>mk\<^isub>o\<^isub>b\<^isub>j\<^isub>e\<^isub>c\<^isub>t oid \<lfloor>_\<rfloor> \<rfloor>\<rfloor> \<Rightarrow> true \<tau>)" 
+
+defs (overloaded) oclistypeof\<^isub>n\<^isub>o\<^isub>d\<^isub>e_Node: 
+        "(X::Node) .oclIsTypeOf(Node) \<equiv> 
+                   (\<lambda>\<tau>. case X \<tau> of 
+                              \<bottom>   \<Rightarrow> invalid \<tau>
+                            | \<lfloor>\<bottom>\<rfloor> \<Rightarrow> invalid \<tau>  
+                            | \<lfloor>\<lfloor> _ \<rfloor>\<rfloor> \<Rightarrow> true \<tau>)"  (* must have actual type Node otherwise  *)
+   
+
+(* MISSING:  Construction for  ocliskind *)
+
+section{* Other operations on states. *}
+(*
 consts oclisnew 
 consts oclismodified 
-consts oclastype 
-consts oclistype
-consts ocliskind
-
 *)
 
 section{* Standard State Infrastructure *}
